scheduler contract obligations

coq/Scheduler/VariableScheduler.v
@@ -789,9 +789,429 @@ Section VariableScheduler.
     | tf_dfg_done => Bits.zero
     end.
 
+  (* ==================================================================== *)
+  (* Helper infrastructure for schedule_no_dup                            *)
+  (* ==================================================================== *)
+
+  (* --- generic list helpers --- *)
+
+  Lemma map_fst_filter_incl {K V} (p: K*V -> bool) (l: list (K*V)) k:
+    In k (map fst (filter p l)) -> In k (map fst l).
+  Proof.
+    induction l as [|[k0 v0] l IH]; simpl; [tauto|].
+    destruct (p (k0,v0)); simpl.
+    - intros [->|Hin]; [left; reflexivity | right; auto].
+    - intro Hin; right; auto.
+  Qed.
+
+  Lemma NoDup_map_fst_filter {K V} (p: K*V -> bool) (l: list (K*V)):
+    NoDup (map fst l) -> NoDup (map fst (filter p l)).
+  Proof.
+    induction l as [|[k0 v0] l IH]; simpl; intro Hnd; [constructor|].
+    inversion Hnd; subst.
+    destruct (p (k0,v0)); simpl.
+    - constructor.
+      + intro Hin. apply map_fst_filter_incl in Hin. contradiction.
+      + apply IH; assumption.
+    - apply IH; assumption.
+  Qed.
+
+  Lemma nodup_map_fst_cons_filter (k: dfg_vars) (v: nid_t) (l: list (dfg_vars * nid_t)):
+    NoDup (map fst l) ->
+    NoDup (map fst ((k,v) :: filter (fun '(k', _) => if eq_dec k' k then false else true) l)).
+  Proof.
+    intro Hnd. simpl. constructor.
+    - intro Hin. apply in_map_iff in Hin. destruct Hin as [[k' v'] [Heq Hin]].
+      simpl in Heq; subst k'. apply filter_In in Hin. destruct Hin as [_ Hp].
+      change ((if eq_dec k k then false else true) = true) in Hp.
+      rewrite eq_dec_refl in Hp. discriminate Hp.
+    - apply NoDup_map_fst_filter; assumption.
+  Qed.
+
+  Lemma list_assoc_none_not_in {K V} `{EqDec K} (l: list (K*V)) (k: K):
+    BitsToLists.list_assoc l k = None -> ~ In k (map fst l).
+  Proof.
+    induction l as [|[k0 v0] l IH]; simpl; [tauto|].
+    destruct (eq_dec k k0) as [->|Hneq].
+    - discriminate.
+    - intros Hnone [Heq|Hin]; [apply Hneq; symmetry; exact Heq | apply IH; assumption].
+  Qed.
+
+  (* --- state-monad invariant plumbing --- *)
+
+  Definition vm_nd (s: dfg_state) : Prop := NoDup (map fst (var_map s)).
+  Definition preserves (P: dfg_state -> Prop) {A} (m: M A) := forall s, P s -> P (snd (m s)).
+
+  Lemma preserves_ret P {A} (x: A): preserves P (ret x).
+  Proof. intros s Hs; exact Hs. Qed.
+
+  Lemma preserves_bind P {A B} (m: M A) (f: A -> M B):
+    preserves P m -> (forall x, preserves P (f x)) -> preserves P (bind m f).
+  Proof.
+    intros Hm Hf s Hs. unfold bind.
+    destruct (m s) as [x s'] eqn:Hms.
+    assert (P s') as Hs'.
+    { specialize (Hm s Hs). rewrite Hms in Hm. exact Hm. }
+    apply (Hf x s' Hs').
+  Qed.
+
+  Lemma emit_vm op sz: preserves vm_nd (emit op sz).
+  Proof.
+    intros s Hs. unfold emit, bind, get_state, put_state, ret; simpl. exact Hs.
+  Qed.
+
+  Lemma ensure_var_vm v: preserves vm_nd (ensure_var v).
+  Proof.
+    intros s Hs. unfold vm_nd, ensure_var.
+    cbn [emit bind get_state put_state ret snd fst var_map].
+    apply nodup_map_fst_cons_filter. exact Hs.
+  Qed.
+
+  Lemma get_var_vm v: preserves vm_nd (get_var v).
+  Proof.
+    intros s Hs. unfold get_var, bind, get_state.
+    destruct (BitsToLists.list_assoc (var_map s) v).
+    - exact Hs.
+    - apply (ensure_var_vm v s Hs).
+  Qed.
+
+  Lemma set_var_vm v id: preserves vm_nd (set_var v id).
+  Proof.
+    intros s Hs. unfold vm_nd, set_var.
+    cbn [bind get_state put_state ret snd fst var_map].
+    apply nodup_map_fst_cons_filter. exact Hs.
+  Qed.
+
+  Lemma dataflow_expr_vm: forall e sz, preserves vm_nd (dataflow_expr e sz).
+  Proof.
+    induction e as [val | sv | iv | ov | uop e IHe
+                    | bop e1 IHe1 e2 IHe2 | ec IHe1 et IHe2 ee IHe3];
+      intros sz; cbn [dataflow_expr].
+    - apply emit_vm.
+    - apply preserves_bind; [apply get_var_vm|]. intro x.
+      destruct (Nat.eqb (dfg_var_size (DFG_SVar sv)) sz); [apply preserves_ret | apply emit_vm].
+    - apply preserves_bind; [apply emit_vm|]. intro x.
+      destruct (Nat.eqb (inputs_var_size iv) sz); [apply preserves_ret | apply emit_vm].
+    - apply preserves_bind; [apply get_var_vm|]. intro x.
+      destruct (Nat.eqb (dfg_var_size (DFG_OVar ov)) sz); [apply preserves_ret | apply emit_vm].
+    - apply preserves_bind; [apply IHe|]. intro x. apply emit_vm.
+    - destruct bop;
+        (apply preserves_bind; [apply IHe1| intro x1;
+         apply preserves_bind; [apply IHe2| intro x2; apply emit_vm]]).
+    - apply preserves_bind; [apply IHe1|]. intro xc.
+      apply preserves_bind; [apply IHe2|]. intro xt.
+      apply preserves_bind; [apply IHe3|]. intro xe. apply emit_vm.
+  Qed.
+
+  Lemma merge_loop_nd cond mt me: forall keys acc s,
+    NoDup (map fst acc) ->
+    NoDup (map fst (fst (merge_loop cond mt me keys acc s))).
+  Proof.
+    induction keys as [|[k kv] rest IH]; intros acc s Hnd; cbn [merge_loop].
+    - exact Hnd.
+    - destruct (BitsToLists.list_assoc acc k) eqn:Ha.
+      + apply IH; exact Hnd.
+      + unfold bind.
+        destruct (merge_key cond k (BitsToLists.list_assoc mt k)
+                    (BitsToLists.list_assoc me k) s) as [res_opt s1].
+        destruct res_opt as [fid|].
+        * apply IH. simpl. constructor.
+          -- apply list_assoc_none_not_in in Ha. exact Ha.
+          -- exact Hnd.
+        * apply IH; exact Hnd.
+  Qed.
+
+  Lemma dataflow_ops_vm: forall ops, preserves vm_nd (dataflow_ops ops).
+  Proof.
+    induction ops as [bop | o1 IHops1 o2 IHops2 | oc ot IHops1 oe IHops2];
+      cbn [dataflow_ops].
+    - destruct bop as [ | dst expr | dst expr].
+      + apply preserves_ret.
+      + apply preserves_bind; [apply dataflow_expr_vm|]. intro x. apply set_var_vm.
+      + apply preserves_bind; [apply dataflow_expr_vm|]. intro x. apply set_var_vm.
+    - apply preserves_bind; [apply IHops1|]. intro x. apply IHops2.
+    - intros s Hs.
+      unfold bind. cbn [get_state put_state].
+      destruct (dataflow_expr oc 1 s) as [xc s0].
+      destruct (dataflow_ops ot s0) as [u1 s1].
+      destruct (dataflow_ops oe {| graph := graph s1; var_map := var_map s0 |}) as [u2 s2].
+      unfold merge_maps, vm_nd.
+      destruct (merge_loop xc (var_map s1) (var_map s2)
+                 (var_map s1 ++ var_map s2) [] s2) as [x0 s3] eqn:Hm.
+      cbn [snd var_map].
+      replace x0 with (fst (merge_loop xc (var_map s1) (var_map s2)
+                 (var_map s1 ++ var_map s2) [] s2)) by (rewrite Hm; reflexivity).
+      apply merge_loop_nd. constructor.
+  Qed.
+
+  Lemma build_dfg_vm a: NoDup (map fst (var_map (build_dfg a))).
+  Proof.
+    unfold build_dfg. simpl.
+    destruct (dataflow_ops (spec_action_ops a)
+                {| graph := [{| nid := 0; op := DFG_Empty; sz := 0 |}]; var_map := [] |})
+      as [u s'] eqn:Hd.
+    simpl.
+    assert (vm_nd s') as Hnd.
+    { pose proof (dataflow_ops_vm (spec_action_ops a)
+        {| graph := [{| nid := 0; op := DFG_Empty; sz := 0 |}]; var_map := [] |}) as Hp.
+      unfold preserves in Hp. specialize (Hp ltac:(unfold vm_nd; simpl; constructor)).
+      rewrite Hd in Hp. exact Hp. }
+    exact Hnd.
+  Qed.
+
+  (* --- generic NoDup-of-flat_map via a key --- *)
+
+  Lemma NoDup_flat_map_key {A B} (f: A -> list B) (l: list A):
+    NoDup l ->
+    (forall x, In x l -> NoDup (f x)) ->
+    (forall x y b, In x l -> In y l -> In b (f x) -> In b (f y) -> x = y) ->
+    NoDup (flat_map f l).
+  Proof.
+    intros Hnd. induction Hnd as [| a l Hnotin Hnd IH]; intros Hin Hkey; simpl.
+    - constructor.
+    - apply NoDup_app.
+      + apply Hin. left. reflexivity.
+      + apply IH.
+        * intros x Hx. apply Hin. right. exact Hx.
+        * intros x y b Hx Hy Hbx Hby.
+          apply (Hkey x y b (or_intror Hx) (or_intror Hy) Hbx Hby).
+      + intros b Hba Hbrest.
+        apply in_flat_map in Hbrest. destruct Hbrest as [y [Hy Hby]].
+        assert (a = y) as Heq
+          by apply (Hkey a y b (or_introl eq_refl) (or_intror Hy) Hba Hby).
+        subst y. contradiction.
+  Qed.
+
+  Lemma nodup_map_inj_in {A K} (g: A -> K) (l: list A):
+    NoDup (map g l) -> forall x y, In x l -> In y l -> g x = g y -> x = y.
+  Proof.
+    induction l as [|a l IH]; intros Hnd x y Hx Hy Hg; [inversion Hx|].
+    simpl in Hnd. inversion Hnd; subst.
+    destruct Hx as [<-|Hx]; destruct Hy as [<-|Hy].
+    - reflexivity.
+    - exfalso. apply H1. rewrite Hg. apply in_map. exact Hy.
+    - exfalso. apply H1. rewrite <- Hg. apply in_map. exact Hx.
+    - apply IH; assumption.
+  Qed.
+
+  Lemma NoDup_flat_map_of_key {A B K} (g: A -> K) (f: A -> list B) (key: B -> K) (l: list A):
+    NoDup (map g l) ->
+    (forall x, In x l -> NoDup (f x)) ->
+    (forall x b, In x l -> In b (f x) -> key b = g x) ->
+    NoDup (flat_map f l).
+  Proof.
+    intros Hnd Hf Hkey. apply NoDup_flat_map_key.
+    - apply NoDup_map_inv with (f:=g); exact Hnd.
+    - exact Hf.
+    - intros x y b Hx Hy Hbx Hby.
+      apply (nodup_map_inj_in g l Hnd x y Hx Hy).
+      rewrite <- (Hkey x b Hx Hbx). rewrite <- (Hkey y b Hy Hby). reflexivity.
+  Qed.
+
+  (* --- get_sizes_and_idx assigns indices 0,1,2,... --- *)
+
+  Lemma fold_idx_map (dfg: dfg_state): forall nodes acc i,
+    map (fun '(_, x) => fst x) (rev (fst (fold_left
+      (fun '(acc0, idx) nid =>
+         let node := nth nid (graph dfg) {| nid := 0; op := DFG_Empty; sz := 0 |} in
+         ((nid, (idx, sz node)) :: acc0, S idx)) nodes (acc, i))))
+    = map (fun '(_, x) => fst x) (rev acc) ++ seq i (length nodes).
+  Proof.
+    induction nodes as [|nid rest IH]; intros acc i.
+    - simpl. rewrite app_nil_r. reflexivity.
+    - cbn [fold_left length]. rewrite IH.
+      cbn [rev]. rewrite map_app. cbn [map]. cbn [seq].
+      rewrite <- app_assoc. reflexivity.
+  Qed.
+
+  Lemma gsi_idx_nodup (dfg: dfg_state) (nodes: list nid_t):
+    NoDup (map (fun '(_, x) => fst x) (get_sizes_and_idx dfg nodes)).
+  Proof.
+    unfold get_sizes_and_idx. rewrite fold_idx_map. simpl. apply seq_NoDup.
+  Qed.
+
+  (* --- flat_map composition helpers --- *)
+
+  Lemma flat_map_flat_map {A B C} (g: B -> list C) (h: A -> list B) (l: list A):
+    flat_map g (flat_map h l) = flat_map (fun x => flat_map g (h x)) l.
+  Proof.
+    induction l as [|a l IH]; simpl; [reflexivity|].
+    rewrite flat_map_app, IH. reflexivity.
+  Qed.
+
+  Lemma flat_map_map {A B C} (f: B -> list C) (g: A -> B) (l: list A):
+    flat_map f (map g l) = flat_map (fun x => f (g x)) l.
+  Proof.
+    induction l as [|a l IH]; simpl; [reflexivity | rewrite IH; reflexivity].
+  Qed.
+
+  Lemma NoDup_map_Some {A} (l: list A): NoDup l -> NoDup (map Some l).
+  Proof.
+    induction 1 as [|x l Hx Hnd IH]; simpl; constructor; [| exact IH].
+    intro Hin. apply in_map_iff in Hin. destruct Hin as [y [Heq Hy]].
+    injection Heq as ->. contradiction.
+  Qed.
+
+  (* --- the op-tag function used by tfs_ops_no_duplicates --- *)
+
+  Notation OPTAG :=
+    (fun op => match op with
+       | tf_assign dst _ => [StOp dst]
+       | tf_output dst _ => [OutOp dst]
+       | _ => []
+       end).
+
+  (* --- buffer-op tags --- *)
+
+  Lemma buffers_tags_in (idx: nat) (DFG: dfg_state)
+        (BUF: list (nid_t * (nat * sz_t))) t:
+    In t (flat_map OPTAG (compile_dfg_buffers idx DFG BUF)) ->
+    exists a' n', t = StOp (tf_dfg_b a' n') \/ t = StOp (tf_dfg_v a' n').
+  Proof.
+    intro Hin. apply in_flat_map in Hin. destruct Hin as [op [Hop Ht]].
+    unfold compile_dfg_buffers in Hop.
+    destruct (index_of_nat (length buffer_needs) idx) as [a'|]; [| destruct Hop].
+    apply in_flat_map in Hop. destruct Hop as [[nid x] [_ Hop]].
+    destruct (index_of_nat _ (fst x)) as [n'|]; [| destruct Hop].
+    match goal with
+    | Hop : In op (let '(_, _) := ?E in _) |- _ =>
+        destruct E as [expr valid]
+    end.
+    simpl in Hop. destruct Hop as [<-|[<-|[]]]; simpl in Ht.
+    - destruct Ht as [<-|[]]. exists a', n'. left. reflexivity.
+    - destruct Ht as [<-|[]]. exists a', n'. right. reflexivity.
+  Qed.
+
+  Lemma buffers_tags_nodup (idx: nat) (DFG: dfg_state)
+        (BUF: list (nid_t * (nat * sz_t))):
+    NoDup (map (fun '(_, x) => fst x) BUF) ->
+    NoDup (flat_map OPTAG (compile_dfg_buffers idx DFG BUF)).
+  Proof.
+    intro HBUF. unfold compile_dfg_buffers.
+    destruct (index_of_nat (length buffer_needs) idx) as [a'|]; [| simpl; constructor].
+    rewrite flat_map_flat_map.
+    apply NoDup_flat_map_of_key
+      with (g := fun '(_, x) => fst x)
+           (key := fun t => match t with
+                    | StOp (tf_dfg_b _ n) => index_to_nat n
+                    | StOp (tf_dfg_v _ n) => index_to_nat n
+                    | _ => 0
+                    end).
+    - exact HBUF.
+    - intros [nid x] _.
+      destruct (index_of_nat _ (fst x)) as [n'|]; [| simpl; constructor].
+      match goal with |- context[let '(_, _) := ?E in _] => destruct E as [expr valid] end.
+      simpl. apply NoDup_cons; [simpl; intros [H|[]]; discriminate H|].
+      apply NoDup_cons; [simpl; tauto | apply NoDup_nil].
+    - intros [nid x] b _ Hb.
+      destruct (index_of_nat _ (fst x)) as [n'|] eqn:Hn; [| destruct Hb].
+      match goal with
+      | Hb : In b (flat_map _ (let '(_, _) := ?E in _)) |- _ =>
+          destruct E as [expr valid]
+      end.
+      simpl in Hb. destruct Hb as [<-|[<-|[]]]; simpl;
+        apply index_to_nat_of_nat in Hn; exact Hn.
+  Qed.
+
+  (* --- final-op tags --- *)
+
+  Lemma final_tags_in (idx: nat) (DFG: dfg_state)
+        (BUF: list (nid_t * (nat * sz_t))) t:
+    In t (flat_map OPTAG (compile_dfg_aux idx DFG BUF)) ->
+    (exists sv, t = StOp (tf_dfg_s sv)) \/ (exists ov, t = OutOp ov).
+  Proof.
+    intro Hin. apply in_flat_map in Hin. destruct Hin as [op [Hop Ht]].
+    unfold compile_dfg_aux in Hop.
+    destruct (index_of_nat (length buffer_needs) idx) as [a'|]; [| destruct Hop].
+    apply in_map_iff in Hop. destruct Hop as [[var nid] [Heq _]].
+    match goal with
+    | Heq : (let '(_, _) := ?E in _) = op |- _ =>
+        destruct E as [expr valid]
+    end.
+    destruct var as [sv|ov]; subst op; simpl in Ht.
+    - destruct Ht as [<-|[]]. left. exists sv. reflexivity.
+    - destruct Ht as [<-|[]]. right. exists ov. reflexivity.
+  Qed.
+
+  Lemma final_tags_nodup (idx: nat) (DFG: dfg_state)
+        (BUF: list (nid_t * (nat * sz_t))):
+    NoDup (map fst (var_map DFG)) ->
+    NoDup (flat_map OPTAG (compile_dfg_aux idx DFG BUF)).
+  Proof.
+    intro HDFG. unfold compile_dfg_aux.
+    destruct (index_of_nat (length buffer_needs) idx) as [a'|]; [| simpl; constructor].
+    rewrite flat_map_map.
+    apply NoDup_flat_map_of_key
+      with (g := fun p => Some (fst p))
+           (key := fun t => match t with
+                    | StOp (tf_dfg_s sv) => Some (DFG_SVar sv)
+                    | OutOp ov => Some (DFG_OVar ov)
+                    | _ => None
+                    end).
+    - rewrite <- (map_map fst Some). apply NoDup_map_Some. exact HDFG.
+    - intros [var nid] _.
+      match goal with |- context[compile_dfg_expr ?f ?a ?d ?n ?b] =>
+        destruct (compile_dfg_expr f a d n b) as [expr valid] end.
+      destruct var as [sv|ov]; simpl; apply NoDup_cons; solve [apply NoDup_nil | simpl; tauto].
+    - intros [var nid] b _ Hb.
+      match goal with
+      | Hb : context[compile_dfg_expr ?f ?a ?d ?n ?bf] |- _ =>
+          destruct (compile_dfg_expr f a d n bf) as [expr valid]
+      end.
+      destruct var as [sv|ov]; simpl in Hb; destruct Hb as [<-|[]]; reflexivity.
+  Qed.
+
+  (* --- assembly --- *)
+
+  Lemma schedule_no_dup_aux (idx: nat) (DFG: dfg_state)
+        (BUF: list (nid_t * (nat * sz_t))):
+    NoDup (map fst (var_map DFG)) ->
+    NoDup (map (fun '(_, x) => fst x) BUF) ->
+    NoDup (flat_map OPTAG
+      ((compile_dfg_valid idx DFG BUF :: compile_dfg_buffers idx DFG BUF)
+       ++ compile_dfg_aux idx DFG BUF)).
+  Proof.
+    intros HDFG HBUF.
+    assert (Hval: flat_map OPTAG
+        (compile_dfg_valid idx DFG BUF :: compile_dfg_buffers idx DFG BUF)
+      = StOp tf_dfg_done :: flat_map OPTAG (compile_dfg_buffers idx DFG BUF)).
+    { unfold compile_dfg_valid. reflexivity. }
+    rewrite flat_map_app, Hval, <- app_comm_cons.
+    apply NoDup_cons.
+    - rewrite in_app_iff. intros [Hb|Hf].
+      + apply buffers_tags_in in Hb. destruct Hb as [a' [n' [Hb|Hb]]]; discriminate Hb.
+      + apply final_tags_in in Hf. destruct Hf as [[sv Hf]|[ov Hf]]; discriminate Hf.
+    - apply NoDup_app.
+      + apply buffers_tags_nodup. exact HBUF.
+      + apply final_tags_nodup. exact HDFG.
+      + intros x Hxb Hxf.
+        apply buffers_tags_in in Hxb. apply final_tags_in in Hxf.
+        destruct Hxb as [a' [n' [-> | ->]]];
+          destruct Hxf as [[sv Hs]|[ov Ho]]; discriminate.
+  Qed.
+
+
   Theorem schedule_no_dup: forall a, tfs_ops_no_duplicates (fst (schedule a) ++ snd (schedule a)).
   Proof.
-  Admitted.
+    intros a. unfold tfs_ops_no_duplicates, schedule. cbn [fst snd].
+    apply schedule_no_dup_aux.
+    - set (i := spec_action_index a).
+      destruct (lt_dec i (length (map build_dfg spec_all_actions))) as [Hlt|Hge].
+      + pose proof (nth_In (map build_dfg spec_all_actions)
+                     {| graph := []; var_map := [] |} Hlt) as HIn.
+        apply in_map_iff in HIn. destruct HIn as [a' [Heq _]].
+        rewrite <- Heq. apply build_dfg_vm.
+      + rewrite nth_overflow by lia. simpl. constructor.
+    - set (i := spec_action_index a).
+      match goal with
+      | |- NoDup (map _ (nth _ ?BUFS _)) =>
+        destruct (lt_dec i (length BUFS)) as [Hlt|Hge];
+        [ pose proof (nth_In BUFS ([]:list (nid_t * (nat * sz_t))) Hlt) as HIn
+        | rewrite nth_overflow by lia; simpl; constructor ]
+      end.
+      apply in_map_iff in HIn. destruct HIn as [[dfg cm] [Heq _]].
+      rewrite <- Heq. apply gsi_idx_nodup.
+  Qed.
 
   Theorem schedule_done_assigned: forall a,    In (StOp done_signal)
        (flat_map (fun op =>
@@ -807,11 +1227,70 @@ Section VariableScheduler.
 
   Theorem reset_states_nodup: NoDup reset_states.
   Proof.
-  Admitted.
+    unfold reset_states.
+    (* recover the a-index and n-index from an element *)
+    pose (a_of := fun v : tf_dfg_states =>
+      match v with
+      | tf_dfg_b a _ => index_to_nat a
+      | tf_dfg_v a _ => index_to_nat a
+      | _ => 0
+      end).
+    pose (n_of := fun v : tf_dfg_states =>
+      match v with
+      | tf_dfg_b _ n => index_to_nat n
+      | tf_dfg_v _ n => index_to_nat n
+      | _ => 0
+      end).
+    apply NoDup_flat_map_key.
+    - apply seq_NoDup.
+    - (* each outer chunk is NoDup *)
+      intros a_idx _.
+      destruct (index_of_nat (length buffer_needs) a_idx) as [a'|] eqn:Ha;
+        [| constructor].
+      apply NoDup_flat_map_key.
+      + apply seq_NoDup.
+      + (* each inner chunk [b; v] is NoDup *)
+        intros n_idx _.
+        destruct (index_of_nat _ n_idx) as [n'|] eqn:Hn; [| constructor].
+        repeat constructor.
+        * simpl. intros [H | []]. discriminate H.
+        * simpl. tauto.
+      + (* inner disjointness: element recovers its n-index *)
+        intros x y b Hx Hy Hbx Hby.
+        assert (forall m b0, In b0 (match index_of_nat _ m with
+                              | Some n' => [tf_dfg_b a' n'; tf_dfg_v a' n']
+                              | None => [] end) -> n_of b0 = m) as Hrec.
+        { intros m b0 Hb0. destruct (index_of_nat _ m) as [n'|] eqn:Hm; [| destruct Hb0].
+          apply index_to_nat_of_nat in Hm.
+          simpl in Hb0. destruct Hb0 as [<- | [<- | []]]; simpl; exact Hm. }
+        rewrite <- (Hrec x b Hbx). rewrite <- (Hrec y b Hby). reflexivity.
+    - (* outer disjointness: element recovers its a-index *)
+      intros x y b Hx Hy Hbx Hby.
+      assert (forall m b0, In b0 (match index_of_nat (length buffer_needs) m with
+                            | Some a' => flat_map (fun n_idx =>
+                                match index_of_nat (length (nth (index_to_nat a') buffer_needs [])) n_idx with
+                                | Some n' => [tf_dfg_b a' n'; tf_dfg_v a' n']
+                                | None => [] end)
+                                (List.seq 0 (length (nth (index_to_nat a') buffer_needs [])))
+                            | None => [] end) -> a_of b0 = m) as Hrec.
+      { intros m b0 Hb0. destruct (index_of_nat (length buffer_needs) m) as [a'|] eqn:Hm;
+          [| destruct Hb0].
+        apply index_to_nat_of_nat in Hm.
+        apply in_flat_map in Hb0. destruct Hb0 as [n_idx [_ Hb0]].
+        destruct (index_of_nat _ n_idx) as [n'|] eqn:Hn; [| destruct Hb0].
+        simpl in Hb0. destruct Hb0 as [<- | [<- | []]]; simpl; exact Hm. }
+      rewrite <- (Hrec x b Hbx). rewrite <- (Hrec y b Hby). reflexivity.
+  Qed.
 
   Theorem reset_states_init_zero: forall v, In v reset_states -> tf_dfg_states_init v = Bits.zero.
   Proof.
-  Admitted.
+    intros v Hin. unfold reset_states in Hin.
+    apply in_flat_map in Hin. destruct Hin as [a_idx [_ Hin]].
+    destruct (index_of_nat (length buffer_needs) a_idx) as [a_idx'|]; [|contradiction].
+    apply in_flat_map in Hin. destruct Hin as [n_idx [_ Hin]].
+    destruct (index_of_nat _ n_idx) as [n_idx'|]; [|contradiction].
+    simpl in Hin. destruct Hin as [<-|[<-|[]]]; reflexivity.
+  Qed.
 
   Definition tfs_schedule : TFSchedule :=
     {|
